src/Assembly/Wordize.v
@@ -1,343 +1,89 @@
-
 Require Export Bedrock.Word Bedrock.Nomega.
 Require Import NArith PArith Ndigits Nnat NPow NPeano Ndec.
 Require Import Compare_dec Omega.
 Require Import FunctionalExtensionality ProofIrrelevance.
 Require Import QhasmUtil QhasmEvalCommon.
-Require Import WordizeUtil.
+Require Import WordizeUtil Bounds Vectorize List.
+
+Import EvalUtil ListNotations.
 
 Hint Rewrite wordToN_nat Nat2N.inj_add N2Nat.inj_add
              Nat2N.inj_mul N2Nat.inj_mul Npow2_nat : N.
 
 Open Scope nword_scope.
 
-Section Wordization.
-  Lemma wordize_plus': forall {n} (x y: word n) (b: N),
-      (b <= Npow2 n)%N
-    -> (&x < b)%N
-    -> (&y < (Npow2 n - b))%N
-    -> (&x + &y)%N = & (x ^+ y).
-  Proof.
-    intros.
-    unfold wplus, wordBin.
-    rewrite wordToN_NToWord; intuition.
-    apply (N.lt_le_trans _ (b + &y)%N _).
+Coercion ind : bool >-> N.
 
-    - apply N.add_lt_le_mono; try assumption; intuition.
-
-    - replace (Npow2 n) with (b + Npow2 n - b)%N by nomega.
-        replace (b + Npow2 n - b)%N with (b + (Npow2 n - b))%N by (
-        replace (b + (Npow2 n - b))%N with ((Npow2 n - b) + b)%N by nomega;
-        rewrite (N.sub_add b (Npow2 n)) by assumption;
-        nomega).
-
-        apply N.add_le_mono_l; try nomega.
-        apply N.lt_le_incl; assumption.
-  Qed.
-
+Section ToWord.
   Lemma wordize_plus: forall {n} (x y: word n),
-    if (overflows n (&x + &y)%N)
-    then (&x + &y)%N = (& (x ^+ y) + Npow2 n)%N
-    else (&x + &y)%N = & (x ^+ y).
+    (&x + &y)%N =
+      if (overflows n (&x + &y)%N)
+      then (& (x ^+ y) + Npow2 n)%N
+      else (& (x ^+ y)).
   Proof. Admitted.
 
   Lemma wordize_awc: forall {n} (x y: word n) (c: bool),
-    if (overflows n (&x + &y + (if c then 1 else 0))%N)
-    then (&x + &y + (if c then 1 else 0))%N = (&(addWithCarry x y c) + Npow2 n)%N
-    else (&x + &y + (if c then 1 else 0))%N = &(addWithCarry x y c).
+    (&x + &y + c)%N =
+      if (overflows n (&x + &y + c)%N)
+      then (&(addWithCarry x y c) + Npow2 n)%N
+      else (&(addWithCarry x y c)).
   Proof. Admitted.
-
-  Lemma wordize_mult': forall {n} (x y: word n) (b: N),
-      (1 < n)%nat -> (0 < b)%N
-    -> (&x < b)%N
-    -> (&y < (Npow2 n) / b)%N
-    -> (&x * &y)%N = & (x ^* y).
-  Proof.
-    intros; unfold wmult, wordBin.
-    rewrite wordToN_NToWord; intuition.
-    apply (N.lt_le_trans _ (b * ((Npow2 n) / b))%N _).
-
-    - apply N.mul_lt_mono; assumption.
-
-    - apply N.mul_div_le; nomega.
-  Qed.
 
   Lemma wordize_mult: forall {n} (x y: word n) (b: N),
     (&x * &y)%N = (&(x ^* y) +
       &((EvalUtil.highBits (n/2) x) ^* (EvalUtil.highBits (n/2) y)) * Npow2 n)%N.
   Proof. intros. Admitted.
 
-  Lemma wordize_and: forall {n} (x y: word n),
-    N.land (&x) (&y) = & (x ^& y).
-  Proof.
-    intros; pose proof (Npow2_gt0 n).
-    pose proof (word_size_bound x).
-    pose proof (word_size_bound y).
-
-    induction n.
-
-    - rewrite (shatter_word_0 x) in *.
-        rewrite (shatter_word_0 y) in *.
-        simpl; intuition.
-
-    - rewrite (shatter_word x) in *.
-        rewrite (shatter_word y) in *.
-        induction (whd x), (whd y).
-
-        + admit.
-        + admit.
-        + admit.
-        + admit.
-  Admitted.
-
   Lemma wordize_shiftr: forall {n} (x: word n) (k: nat),
     (N.shiftr_nat (&x) k) = & (shiftr x k).
   Proof. Admitted.
+End ToWord.
 
-End Wordization.
-
-Section Bounds.
-
-  Theorem constant_bound_N : forall {n} (k: word n),
-    (& k < & k + 1)%N.
-  Proof. intros; nomega. Qed.
-
-  Theorem constant_bound_nat : forall (n k: nat),
-      (N.of_nat k < Npow2 n)%N
-    -> (& (@natToWord n k) < (N.of_nat k) + 1)%N.
-  Proof.
-    intros.
-    rewrite wordToN_nat.
-    rewrite wordToNat_natToWord_idempotent;
-      try assumption; nomega.
-  Qed.
-
-  Lemma let_bound : forall {n} (x: word n) (f: word n -> word n) xb fb,
-      (& x < xb)%N
-    -> (forall x', & x' < xb -> & (f x') < fb)%N
-    -> ((let k := x in &(f k)) < fb)%N.
-  Proof. intros; eauto. Qed.
-
-  Definition Nlt_dec (x y: N): {(x < y)%N} + {(x >= y)%N}.
-    refine (
-      let c := N.compare x y in
-      match c as c' return c = c' -> _ with
-      | Lt => fun _ => left _
-      | _ => fun _ => right _
-      end eq_refl);
-    abstract (
-      unfold c, N.ge, N.lt in *; intuition; subst;
-      match goal with
-      | [H0: ?x = _, H1: ?x = _ |- _] =>
-        rewrite H0 in H1; inversion H1
-      end).
-  Defined.
-
-  Theorem wplus_bound : forall {n} (w1 w2 : word n) b1 b2,
-      (&w1 < b1)%N
-    -> (&w2 < b2)%N
-    -> (&(w1 ^+ w2) < b1 + b2)%N.
-  Proof.
-    intros.
-
-    destruct (Nlt_dec (b1 + b2)%N (Npow2 n));
-      rewrite <- wordize_plus' with (b := b1);
-      try apply N.add_lt_mono;
-      try assumption.
-
-    (* A couple inequality subgoals *)
-  Admitted.
-
-  Theorem wmult_bound : forall {n} (w1 w2 : word n) b1 b2,
-      (1 < n)%nat
-    -> (&w1 < b1)%N
-    -> (&w2 < b2)%N
-    -> (&(w1 ^* w2) < b1 * b2)%N.
-  Proof.
-    intros.
-    destruct (Nlt_dec (b1 * b2)%N (Npow2 n));
-      rewrite <- wordize_mult' with (b := b1);
-      try apply N.mul_lt_mono;
-      try assumption;
-      try nomega.
-
-    (* A couple inequality subgoals *)
-  Admitted.
-
-  Theorem shiftr_bound : forall {n} (w : word n) b bits,
-      (&w < b)%N
-    -> (&(shiftr w bits) < N.succ (N.shiftr_nat b bits))%N.
-  Proof.
-    intros.
-    assert (& shiftr w bits <= N.shiftr_nat b bits)%N. {
-      rewrite <- wordize_shiftr.
-      induction bits; unfold N.shiftr_nat in *; simpl; intuition.
-
-      - unfold N.le, N.lt in *; rewrite H; intuition; inversion H0.
-
-      - revert IHbits;
-
-       admit. (* Monotonicity of N.div2 *)
-    }
-
-    apply N.le_lteq in H0; destruct H0; nomega.
-  Admitted.
-
-  Theorem mask_bound : forall {n} (w : word n) m,
-    (n > 1)%nat ->
-    (&(mask m w) < Npow2 m)%N.
-  Proof.
-    intros.
-    unfold mask in *; destruct (le_dec m n); simpl;
-      try apply extend_bound.
-
-    pose proof (word_size_bound w).
-    apply (N.le_lt_trans _ (Npow2 n) _).
-
-    - unfold N.le, N.lt in *; rewrite H0; intuition; inversion H1.
-
-    - clear H H0.
-      replace m with ((m - n) + n) by nomega.
-      replace (Npow2 n) with (1 * (Npow2 n))%N
-        by (rewrite N.mul_comm; nomega).
-      rewrite Npow2_split.
-      apply N.mul_lt_mono_pos_r.
-
-      + apply Npow2_gt0.
-
-      + assert (0 < m - n)%nat by omega.
-        induction (m - n); try inversion H; try abstract (
-          simpl; replace 2 with (S 1) by omega;
-          apply N.lt_1_2).
-
-        assert (0 < n1)%nat as Z by omega; apply IHn1 in Z.
-        apply (N.le_lt_trans _ (Npow2 n1) _).
-
-        * admit.
-        * admit.
-  Admitted.
-
-  Theorem mask_update_bound : forall {n} (w : word n) b m,
-      (n > 1)%nat
-    -> (&w < b)%N
-    -> (&(mask m w) < (N.min b (Npow2 m)))%N.
-  Proof.
-    intros; unfold mask, N.min;
-      destruct (le_dec m n),
-               (N.compare b (Npow2 m));
-      simpl; try assumption.
-
-  Admitted.
-
-End Bounds.
+Definition wordeq {ins outs} (n: nat) (f: Curried N N ins outs) :=
+  {g: Curried (word n) (word n) ins outs |
+   forall (x: list (word n)), length x = ins ->
+      map (@wordToN n) ((curriedToList (wzero _) g) x) =
+        (curriedToList 0%N f) (map (@wordToN n) x)}.
 
 (** Wordization Tactics **)
 
-Ltac wordize_ast :=
+Ltac wordize_iter :=
   repeat match goal with
-  | [ H: (& ?x < ?b)%N |- context[((& ?x) + (& ?y))%N] ] => rewrite (wordize_plus' x y b)
-  | [ H: (& ?x < ?b)%N |- context[((& ?x) * (& ?y))%N] ] => rewrite (wordize_mult' x y b)
-  | [ |- context[N.land (& ?x) (& ?y)] ] => rewrite (wordize_and x y)
+  | [ |- context[overflows ?n ?x] ] => destruct (overflows n x)
+  | [ |- context[& ?x + & ?y + ind ?b] ] => rewrite wordize_awc
+  | [ |- context[N.mul (& ?x) (& ?y)] ] => rewrite wordize_mult
+  | [ |- context[N.add (& ?x) (& ?y)] ] => rewrite wordize_plus
+  | [ |- context[N.land (& ?x) _] ] => rewrite <- mask_spec
   | [ |- context[N.shiftr (& ?x) ?k] ] => rewrite (wordize_shiftr x k)
-  | [ |- (_ < _ / _)%N ] => unfold N.div; simpl
-  | [ |- context[Npow2 _] ] => simpl
-  | [ |- (?x < ?c)%N ] => assumption
   | [ |- _ = _ ] => reflexivity
+  end.
+
+Ltac wordize_intro :=
+  repeat eexists; intros; list_destruct; simpl.
+
+Ltac wordize_contra :=
+  match goal with
+  | [ H: (_ >= _)%N |- _ ] =>
+    unfold N.ge in H;
+      contradict H;
+      apply N.compare_lt_iff
   end.
 
 Ltac lt_crush := try abstract (clear; vm_compute; intuition).
 
-(** Bounding Tactics **)
-
-Ltac multi_apply0 A L := pose proof (L A).
-
-Ltac multi_apply1 A L :=
-  match goal with
-  | [ H: A < ?b |- _] => pose proof (L A b H)
-  end.
-
-Ltac multi_apply2 A B L :=
-  match goal with
-  | [ H1: A < ?b1, H2: B < ?b2 |- _] => pose proof (L A B b1 b2 H1 H2)
-  end.
-
-Ltac multi_recurse n T :=
-  match goal with
-  | [ H: (T < _)%N |- _] => idtac
-  | _ =>
-    is_var T;
-    let T' := (eval cbv delta [T] in T) in multi_recurse n T';
-    match goal with
-    | [ H : T' < ?x |- _ ] =>
-      pose proof (H : T < x)
-    end
-
-  | _ =>
-    match T with
-    | ?W1 ^+ ?W2 =>
-      multi_recurse n W1; multi_recurse n W2;
-      multi_apply2 W1 W2 (@wplus_bound n)
-
-    | ?W1 ^* ?W2 =>
-      multi_recurse n W1; multi_recurse n W2;
-      multi_apply2 W1 W2 (@wmult_bound n)
-
-    | mask ?m ?w =>
-      multi_recurse n w;
-      multi_apply1 w (fun b => @mask_update_bound n w b)
-
-    | mask ?m ?w =>
-      multi_recurse n w;
-      pose proof (@mask_bound n w m)
-
-    | ?x ^& (@NToWord _ (N.ones ?m)) =>
-      multi_recurse n (mask (N.to_nat m) x);
-      match goal with
-      | [ H: (& (mask (N.to_nat m) x) < ?b)%N |- _] =>
-        pose proof (@mask_wand n x m b H)
-      end
-
-    | shiftr ?w ?bits =>
-      multi_recurse n w;
-      match goal with
-      | [ H: (w < ?b)%N |- _] =>
-        pose proof (@shiftr_bound n w b bits H)
-      end
-
-    | NToWord _ ?k => pose proof (@constant_bound_N n k)
-    | natToWord _ ?k => pose proof (@constant_bound_nat n k)
-    | _ => pose proof (@word_size_bound n T)
-    end
-  end.
-
-Lemma unwrap_let: forall {n} (y: word n) (f: word n -> word n) (b: N),
-    (&(let x := y in f x) < b)%N <-> let x := y in (&(f x) < b)%N.
-Proof. intuition. Qed.
-
-Ltac multi_bound n :=
-  match goal with
-  | [|- let A := ?B in _] =>
-    multi_recurse n B; intro; multi_bound n
-  | [|- ((let A := _ in _) < _)%N] =>
-    apply unwrap_let; multi_bound n
-  | [|- (?W < _)%N ] =>
-    multi_recurse n W
-  end.
-
 (** Examples **)
 
 Module WordizationExamples.
+  Definition example0 : Curried N N 2 1 := fun x y =>
+    N.add (N.land x (N.ones 16)) (N.land y (N.ones 16)).
 
-  Lemma wordize_example0: forall (x y z: word 16),
-    (wordToN x < 10)%N ->
-    (wordToN y < 10)%N ->
-    (wordToN z < 10)%N ->
-    & (x ^* y) = (&x * &y)%N.
+  Lemma wordize_example0: wordeq 16 example0.
   Proof.
-    intros.
-    wordize_ast; lt_crush.
-    transitivity 10%N; try assumption; lt_crush.
-  Qed.
+    unfold example0.
+    wordize_intro.
+    wordize_iter.
+    wordize_contra.
+  Admitted.
 
 End WordizationExamples.
 
