src/Assembly/Bounds.v
@@ -1,0 +1,244 @@
+Require Export Bedrock.Word Bedrock.Nomega.
+Require Import NArith PArith Ndigits Nnat NPow NPeano Ndec.
+Require Import Compare_dec Omega.
+Require Import FunctionalExtensionality ProofIrrelevance.
+Require Import QhasmUtil QhasmEvalCommon.
+Require Import WordizeUtil Vectorize.
+
+Import EvalUtil.
+
+Hint Rewrite wordToN_nat Nat2N.inj_add N2Nat.inj_add
+             Nat2N.inj_mul N2Nat.inj_mul Npow2_nat : N.
+
+Open Scope nword_scope.
+
+Section Bounds.
+  Lemma wordize_plus': forall {n} (x y: word n) (b: N),
+      (b <= Npow2 n)%N
+    -> (&x < b)%N
+    -> (&y < (Npow2 n - b))%N
+    -> (&x + &y)%N = & (x ^+ y).
+  Proof.
+    intros.
+    unfold wplus, wordBin.
+    rewrite wordToN_NToWord; intuition.
+    apply (N.lt_le_trans _ (b + &y)%N _).
+
+    - apply N.add_lt_le_mono; try assumption; intuition.
+
+    - replace (Npow2 n) with (b + Npow2 n - b)%N by nomega.
+        replace (b + Npow2 n - b)%N with (b + (Npow2 n - b))%N by (
+        replace (b + (Npow2 n - b))%N with ((Npow2 n - b) + b)%N by nomega;
+        rewrite (N.sub_add b (Npow2 n)) by assumption;
+        nomega).
+
+        apply N.add_le_mono_l; try nomega.
+        apply N.lt_le_incl; assumption.
+  Qed.
+
+  Lemma wordize_mult': forall {n} (x y: word n) (b: N),
+      (1 < n)%nat -> (0 < b)%N
+    -> (&x < b)%N
+    -> (&y < (Npow2 n) / b)%N
+    -> (&x * &y)%N = & (x ^* y).
+  Proof.
+    intros; unfold wmult, wordBin.
+    rewrite wordToN_NToWord; intuition.
+    apply (N.lt_le_trans _ (b * ((Npow2 n) / b))%N _).
+
+    - apply N.mul_lt_mono; assumption.
+
+    - apply N.mul_div_le; nomega.
+  Qed.
+
+  Theorem constant_bound_N : forall {n} (k: word n),
+    (& k < & k + 1)%N.
+  Proof. intros; nomega. Qed.
+
+  Theorem constant_bound_nat : forall (n k: nat),
+      (N.of_nat k < Npow2 n)%N
+    -> (& (@natToWord n k) < (N.of_nat k) + 1)%N.
+  Proof.
+    intros.
+    rewrite wordToN_nat.
+    rewrite wordToNat_natToWord_idempotent;
+      try assumption; nomega.
+  Qed.
+
+  Lemma let_bound : forall {n} (x: word n) (f: word n -> word n) xb fb,
+      (& x < xb)%N
+    -> (forall x', & x' < xb -> & (f x') < fb)%N
+    -> ((let k := x in &(f k)) < fb)%N.
+  Proof. intros; eauto. Qed.
+
+  Definition Nlt_dec (x y: N): {(x < y)%N} + {(x >= y)%N}.
+    refine (
+      let c := N.compare x y in
+      match c as c' return c = c' -> _ with
+      | Lt => fun _ => left _
+      | _ => fun _ => right _
+      end eq_refl);
+    abstract (
+      unfold c, N.ge, N.lt in *; intuition; subst;
+      match goal with
+      | [H0: ?x = _, H1: ?x = _ |- _] =>
+        rewrite H0 in H1; inversion H1
+      end).
+  Defined.
+
+  Theorem wplus_bound : forall {n} (w1 w2 : word n) b1 b2,
+      (&w1 < b1)%N
+    -> (&w2 < b2)%N
+    -> (&(w1 ^+ w2) < b1 + b2)%N.
+  Proof.
+    intros.
+
+    destruct (Nlt_dec (b1 + b2)%N (Npow2 n));
+      rewrite <- wordize_plus' with (b := b1);
+      try apply N.add_lt_mono;
+      try assumption.
+
+    (* A couple inequality subgoals *)
+  Admitted.
+
+  Theorem wmult_bound : forall {n} (w1 w2 : word n) b1 b2,
+      (1 < n)%nat
+    -> (&w1 < b1)%N
+    -> (&w2 < b2)%N
+    -> (&(w1 ^* w2) < b1 * b2)%N.
+  Proof.
+    intros.
+    destruct (Nlt_dec (b1 * b2)%N (Npow2 n));
+      rewrite <- wordize_mult' with (b := b1);
+      try apply N.mul_lt_mono;
+      try assumption;
+      try nomega.
+
+    (* A couple inequality subgoals *)
+  Admitted.
+
+  Theorem shiftr_bound : forall {n} (w : word n) b bits,
+      (&w < b)%N
+    -> (&(shiftr w bits) < N.succ (N.shiftr_nat b bits))%N.
+  Proof.
+    intros.
+    assert (& shiftr w bits <= N.shiftr_nat b bits)%N. {
+  Admitted.
+
+  Theorem mask_bound : forall {n} (w : word n) m,
+    (n > 1)%nat ->
+    (&(mask m w) < Npow2 m)%N.
+  Proof.
+    intros.
+    unfold mask in *; destruct (le_dec m n); simpl;
+      try apply extend_bound.
+
+    pose proof (word_size_bound w).
+    apply (N.le_lt_trans _ (Npow2 n) _).
+
+    - unfold N.le, N.lt in *; rewrite H0; intuition; inversion H1.
+
+    - clear H H0.
+      replace m with ((m - n) + n) by nomega.
+      replace (Npow2 n) with (1 * (Npow2 n))%N
+        by (rewrite N.mul_comm; nomega).
+      rewrite Npow2_split.
+      apply N.mul_lt_mono_pos_r.
+
+      + apply Npow2_gt0.
+
+      + assert (0 < m - n)%nat by omega.
+        induction (m - n); try inversion H; try abstract (
+          simpl; replace 2 with (S 1) by omega;
+          apply N.lt_1_2).
+
+        assert (0 < n1)%nat as Z by omega; apply IHn1 in Z.
+        apply (N.le_lt_trans _ (Npow2 n1) _).
+
+        * admit.
+        * admit.
+  Admitted.
+
+  Theorem mask_update_bound : forall {n} (w : word n) b m,
+      (n > 1)%nat
+    -> (&w < b)%N
+    -> (&(mask m w) < (N.min b (Npow2 m)))%N.
+  Proof.
+    intros; unfold mask, N.min;
+      destruct (le_dec m n),
+               (N.compare b (Npow2 m));
+      simpl; try assumption.
+
+  Admitted.
+
+End Bounds.
+
+(** Bounding Tactics **)
+
+Ltac multi_apply0 A L := pose proof (L A).
+
+Ltac multi_apply1 A L :=
+  match goal with
+  | [ H: A < ?b |- _] => pose proof (L A b H)
+  end.
+
+Ltac multi_apply2 A B L :=
+  match goal with
+  | [ H1: A < ?b1, H2: B < ?b2 |- _] => pose proof (L A B b1 b2 H1 H2)
+  end.
+
+Ltac multi_recurse n T :=
+  match goal with
+  | [ H: (T < _)%N |- _] => idtac
+  | _ =>
+    is_var T;
+    let T' := (eval cbv delta [T] in T) in multi_recurse n T';
+    match goal with
+    | [ H : T' < ?x |- _ ] =>
+      pose proof (H : T < x)
+    end
+
+  | _ =>
+    match T with
+    | ?W1 ^+ ?W2 =>
+      multi_recurse n W1; multi_recurse n W2;
+      multi_apply2 W1 W2 (@wplus_bound n)
+
+    | ?W1 ^* ?W2 =>
+      multi_recurse n W1; multi_recurse n W2;
+      multi_apply2 W1 W2 (@wmult_bound n)
+
+    | mask ?m ?w =>
+      multi_recurse n w;
+      multi_apply1 w (fun b => @mask_update_bound n w b)
+
+    | mask ?m ?w =>
+      multi_recurse n w;
+      pose proof (@mask_bound n w m)
+
+    | shiftr ?w ?bits =>
+      multi_recurse n w;
+      match goal with
+      | [ H: (w < ?b)%N |- _] =>
+        pose proof (@shiftr_bound n w b bits H)
+      end
+
+    | NToWord _ ?k => pose proof (@constant_bound_N n k)
+    | natToWord _ ?k => pose proof (@constant_bound_nat n k)
+    | _ => pose proof (@word_size_bound n T)
+    end
+  end.
+
+Lemma unwrap_let: forall {n} (y: word n) (f: word n -> word n) (b: N),
+    (&(let x := y in f x) < b)%N <-> let x := y in (&(f x) < b)%N.
+Proof. intuition. Qed.
+
+Ltac multi_bound n :=
+  match goal with
+  | [|- let A := ?B in _] =>
+    multi_recurse n B; intro; multi_bound n
+  | [|- ((let A := _ in _) < _)%N] =>
+    apply unwrap_let; multi_bound n
+  | [|- (?W < _)%N ] =>
+    multi_recurse n W
+  end.
